---
title: 'Analytic Expressions of Indices for the Upper-triangle Matrix'
date: 2020-03-07
permalink: /blogs/indices-for-the-upper-triangle-matrix/
tags:
  - CS
summary: ""
---

Recently, I implemented the negative edge sampling of undirected graphs for [PyTorch Geometric](https://pytorch-geometric.readthedocs.io/). Since $(i, j)$ and $(j, i)$ are the same edge in the undirected graph, I sample entries from the upper triangle of the given adjacency matrix. Easy solution is using [`numpy.triu_indices`](https://docs.scipy.org/doc/numpy/reference/generated/numpy.triu_indices.html), but this suffers from $O(N^2)$ memory complexity (for $G = (V, E)$ and $N = \|V\|$) from the possible edge space $V \times V$.

For the negative sampling of directed graphs, the existing code of PyTorch Geometric first converts the coordinates $(i, j)$ to linear (or consecutive) indices $N \cdot i + j$ and samples indices from $\[ 0, N^2 - 1 \]$ (`range(N ** 2)`). Note that using python standard `random.sample` with `range` is really memory-efficient as the [docs](https://docs.python.org/3/library/random.html#random.sample) says.

In order to apply this to the undirected version of negative sampling, we need to convert the upper triangle matrix into linear indices. For example, the linear indices of the $N = 4$ graph's upper triangle matrix will be:
```
0  1  2  3
-  4  5  6
-  -  7  8
-  -  -  9
```

Encoding the coordinate $(i, j)$ to the linear index $X$ is straightforward. The cumulative number of neglected entries for the $i$th row is $\sum_{x=0}^{i} x = \frac{i (i + 1)}{2}$, so substracting this value to the indices of the original matrix will be the solution.

$X = Ni + j - \frac{i (i + 1)}{2}$.

What about the inverse? Can we infer $i$ and $j$ from $X$? The answer is yes. There are analytic expressions of $i$ and $j$ in terms of $X$, and actually are well known results in StackOverflow [[1](https://stackoverflow.com/a/53234021), [2](https://stackoverflow.com/a/244550)].

$i = N - 1 - \left[\frac{-1 + \sqrt{(2N+1)^2 - 8 (X + 1)}}{2} \right]$

$j = X - Ni + \frac{i (i + 1)}{2}$

```python
i = N - 1 - np.floor((-1 + np.sqrt((2 * N + 1) ** 2 - 8 * (X + 1))) / 2)
j = X - i * (2 * N - i - 1) // 2
```

My sincere friend, Chaehwan Song, explained to me how the above equations are derived. With her permission, I describe her solution in this post.

![upper-matrix](/images/upper-matrix.png)

The size of the shaded area is $\sum_{z=1}^{N} z - (X + 1) = \frac{N(N+1)}{2} - (X + 1)$, and from the right figure, we know that the following equation holds.

$\sum_{z=1}^{N - 1 - i} z \leq \frac{N(N+1)}{2} - (X + 1) < \sum_{z=1}^{N - i} z$

$\Rightarrow \frac{(N-1-i)(N-i)}{2} \leq \frac{N(N+1)}{2} - (X + 1) < \frac{(N-i)(N-i+1)}{2}$ (①)

Let $i^c = N - 1 - i$ (for simplicity), $f(x) = \frac{x(x+1)}{2}$, and $k \in [0, N]$ s.t. $f(k) = \frac{N(N+1)}{2} - X$.

Then, equation ① becomes $f(i^c) \leq f(k) < f(i^c + 1)$.

Since $f(x)$ is monotically increasing at $[0, N]$, we obatin $i^c \leq k < i^c + 1$, which directly implies that $[ k ] = i^c$ holds (②).

From the definition of $k$,

$f(k) = \frac{k(k+1)}{2} = \frac{N(N+1)}{2} - (X + 1)$

$\Rightarrow k = \frac{-1 \pm \sqrt{(2N+1)^2 - 8 (X + 1)}}{2}$,

and proper $k \in [0, N]$ is $k = \frac{-1 + \sqrt{(2N+1)^2 - 8 (X + 1)}}{2}$.

From ②, we have $i^c = \left[ \frac{-1 + \sqrt{(2N+1)^2 - 8 (X + 1)}}{2} \right]$.

$\therefore i = N - 1 - \left[\frac{-1 + \sqrt{(2N+1)^2 - 8 (X + 1)}}{2} \right]$,

and $j$ follows in a straightforward way.